Phi_System/Phi_Fictions.thy
@@ -2,6 +2,24 @@ theory Phi_Fictions
   imports Phi_Types
 begin
 
+definition refinement_projection :: \<open>('abstract::sep_magma \<Rightarrow> 'concrete BI) \<Rightarrow> 'abstract set \<Rightarrow> 'concrete set\<close>
+  where \<open>refinement_projection I D = Sup ((BI.dest o I) ` (D * top))\<close>
+
+lemma refinement_projection_mono:
+  \<open> D \<le> D'
+\<Longrightarrow> refinement_projection I D \<le> refinement_projection I D'\<close>
+  unfolding refinement_projection_def
+  by (clarsimp simp add: less_eq_BI_iff set_mult_expn Bex_def; blast)
+
+lemma set_top_times_idem:
+  \<open>top * top = (top :: 'a::sep_magma_1 set)\<close>
+  unfolding set_eq_iff
+  by (clarsimp simp: set_mult_expn, metis mult_1_class.mult_1_right sep_magma_1_left)
+
+lemma refinement_projection_UNIV_times_D[simp]:
+  \<open> refinement_projection I (D * top) \<le> refinement_projection I D \<close>
+  for D :: \<open>'a::sep_monoid set\<close>
+  unfolding refinement_projection_def mult.assoc set_top_times_idem ..
 
 
 subsection \<open>Instances\<close>
@@ -12,17 +30,19 @@ lemma Itself_refinement_projection:
   \<open> S \<le> S'
 \<Longrightarrow> refinement_projection Itself S \<le> S' * top\<close>
   unfolding refinement_projection_def
-  by (clarsimp simp add: less_eq_BI_iff) blast
+  by (clarsimp simp add: set_mult_expn, blast)
 
 lemma Itself_refinement:
-  \<open>((u,v) \<Ztypecolon> Itself) * BI_Id_on top \<r>\<e>\<f>\<i>\<n>\<e>\<s> (u,v) \<Ztypecolon> Itself \<w>.\<r>.\<t> Itself \<i>\<n> (u \<Ztypecolon> Itself)\<close>
+  \<open>{(u,v)} * Id_on top \<r>\<e>\<f>\<i>\<n>\<e>\<s> {(u,v)} \<w>.\<r>.\<t> Itself \<i>\<n> {u}\<close>
   for u :: \<open>'a::{sep_cancel,sep_semigroup}\<close>
   unfolding Fictional_Forward_Simulation_def
-  by (clarsimp simp add: less_eq_BI_iff,
+  by (clarsimp simp add: subset_iff set_mult_expn,
       metis sep_cancel sep_disj_multD1 sep_disj_multD2 sep_disj_multI1 sep_disj_multI2 sep_mult_assoc)
 
 
 subsubsection \<open>Composition\<close>
+
+
 
 
 lemma sep_refinement_stepwise:
@@ -35,9 +55,7 @@ lemma sep_refinement_stepwise:
   apply (auto simp add: subset_iff Image_def Bex_def less_eq_BI_iff set_mult_expn split_option_all)
   subgoal premises prems for x r R t u v xb
   proof -
-    thm prems
-    thm prems(1)[THEN spec[where x=xb],THEN spec[where x=1],THEN spec[where x=\<open>R\<close>],THEN spec[where x=\<open>t\<close>]]
-    have \<open>\<exists>w'. (w', t) \<Turnstile> S1 \<and> (\<exists>u v. w' = u * v \<and> u \<Turnstile> Ia (xb * 1) \<and> v \<Turnstile> R \<and> u ## v) \<and> xb ## 1 \<and> xb \<Turnstile> D\<close>
+    have \<open>\<exists>x. (\<exists>u v. x = u * v \<and> u \<Turnstile> Ia (xb * 1) \<and> v \<Turnstile> R \<and> u ## v) \<and> xb ## 1 \<and> xb \<in> D \<and> (x, t) \<in> S1\<close>
       using prems(10) prems(3) prems(4) prems(5) prems(6) prems(7) prems(8) prems(9) by fastforce
     note prems(1)[THEN spec[where x=xb],THEN spec[where x=1],THEN spec[where x=\<open>R\<close>],THEN spec[where x=\<open>t\<close>],
           THEN mp, OF this]
@@ -45,7 +63,7 @@ lemma sep_refinement_stepwise:
       apply clarsimp
       subgoal premises prems2 for y u'' v''
       proof -
-        have \<open>\<exists>w'. (w', y) \<Turnstile> S2 \<and> (\<exists>u v. w' = u * v \<and> u \<Turnstile> Ib (x * r) \<and> v \<Turnstile> Itself 1 \<and> u ## v) \<and> x ## r \<and> x \<Turnstile> D'\<close>
+        have \<open>\<exists>xa. (\<exists>u v. xa = u * v \<and> u \<Turnstile> Ib (x * r) \<and> v \<Turnstile> Itself 1 \<and> u ## v) \<and> x ## r \<and> x \<in> D' \<and> (xa, y) \<in> S2\<close>
           by (simp, rule exI[where x=xb], simp add: prems2 prems)
         note prems(2)[THEN spec[where x=x],THEN spec[where x=r],THEN spec[where x=\<open>Itself 1\<close>], THEN spec[where x=y],
                 THEN mp, OF this]
@@ -137,16 +155,16 @@ lemma \<F>_pointwise_Itself:
 
 lemma \<F>_pointwise_projection:
   \<open> refinement_projection (I k) D' \<le> D * top
-\<Longrightarrow> refinement_projection (\<F>_pointwise I) (fun_upd 1 k `\<^sub>I D') \<le> fun_upd 1 k `\<^sub>I D * top\<close>
-  for D :: \<open>'b::sep_monoid BI\<close>
-  apply (clarsimp simp add: less_eq_BI_iff Bex_def image_iff set_mult_expn times_fun
+\<Longrightarrow> refinement_projection (\<F>_pointwise I) (fun_upd 1 k ` D') \<le> fun_upd 1 k ` D * top\<close>
+  for D :: \<open>'b::sep_monoid set\<close>
+  apply (clarsimp simp add: subset_iff Bex_def image_iff set_mult_expn times_fun
             refinement_projection_def)
   subgoal premises prems for t u xb
   proof -
     have t1: \<open>xb ## u k\<close>
       by (metis fun_upd_same prems(3) sep_disj_fun)
-    have \<open>\<exists>m. (\<exists>w'. m = I k w' \<and> (\<exists>u v. w' = u * v \<and> u \<Turnstile> D' \<and> u ## v)) \<and> t k \<Turnstile> m\<close>
-      by (metis prems(2) prems(4) t1)
+    have \<open>\<exists>x. (\<exists>xa. (\<exists>u v. xa = u * v \<and> u \<in> D' \<and> u ## v) \<and> x = BI.dest (I k xa)) \<and> t k \<in> x\<close>
+      by (metis Satisfaction_def prems(2) prems(4) t1)
     note prems(1)[THEN spec[where x=\<open>t k\<close>], THEN mp, OF this]
     then show ?thesis
       apply clarsimp
@@ -156,23 +174,24 @@ lemma \<F>_pointwise_projection:
   qed .
 
 lemma \<F>_pointwise_refinement:
-  \<open> A * BI_Id_on top \<r>\<e>\<f>\<i>\<n>\<e>\<s> B \<w>.\<r>.\<t> I k \<i>\<n> D
-\<Longrightarrow> pairself (fun_upd 1 k) `\<^sub>I A * BI_Id_on top \<r>\<e>\<f>\<i>\<n>\<e>\<s> pairself (fun_upd 1 k) `\<^sub>I B
-    \<w>.\<r>.\<t> \<F>_pointwise I \<i>\<n> fun_upd 1 k `\<^sub>I D\<close>
+  \<open> A * Id_on top \<r>\<e>\<f>\<i>\<n>\<e>\<s> B \<w>.\<r>.\<t> I k \<i>\<n> D
+\<Longrightarrow> pairself (fun_upd 1 k) ` A * Id_on top \<r>\<e>\<f>\<i>\<n>\<e>\<s> pairself (fun_upd 1 k) ` B
+    \<w>.\<r>.\<t> \<F>_pointwise I \<i>\<n> fun_upd 1 k ` D\<close>
   for I :: \<open>'c \<Rightarrow> 'b::sep_magma_1 \<Rightarrow> 'a::sep_magma_1 BI\<close>
   unfolding Fictional_Forward_Simulation_def
-  apply (clarsimp simp add: set_mult_expn image_iff Image_def less_eq_BI_iff Bex_def times_fun Id_on_iff)
-  subgoal premises prems for r R xc u v xb a b
+  apply (clarsimp simp add: set_mult_expn image_iff Image_def subset_iff Bex_def times_fun Id_on_iff)
+  subgoal premises prems for r R u v xb xc a b
   proof -
+thm prems
     have t1[simp]: \<open>a ## xc k\<close>
       by (metis fun_upd_same prems(8) sep_disj_fun)
     have t2[simp]: \<open>b ## xc k\<close>
       by (metis fun_upd_same prems(9) sep_disj_fun)
-    have \<open>\<exists>w'. (\<exists>a ba aa. w' = a * aa \<and> b * xc k = ba * aa \<and> (a, ba) \<Turnstile> A \<and> a ## aa \<and> ba ## aa) \<and>
-      (\<exists>u va. w' = u * va \<and> u \<Turnstile> I k (xb * r k) \<and> va \<Turnstile> Itself (v k) \<and> u ## va) \<and> xb ## r k \<and> xb \<Turnstile> D\<close>
+    have \<open>\<exists>x. (\<exists>u va. x = u * va \<and> u \<Turnstile> I k (xb * r k) \<and> va \<Turnstile> Itself (v k) \<and> u ## va) \<and>
+     xb ## r k \<and> xb \<in> D \<and> (\<exists>a ba aa. x = a * aa \<and> b * xc k = ba * aa \<and> (a, ba) \<in> A \<and> a ## aa \<and> ba ## aa)\<close>
       by (auto simp add: prems,
           smt (verit, ccfv_threshold) fun_upd_same prems(10) prems(2) prems(3) prems(5) prems(7) sep_disj_fun_def t1 t2 times_fun_def)
-    note prems(1)[THEN spec[where x=xb], THEN spec[where x=\<open>r k\<close>], THEN spec[where x=\<open>Itself (v k)\<close>, THEN spec[where x=\<open>b * xc k\<close>]],
+    note prems(1)[THEN spec[where x=xb], THEN spec[where x=\<open>r k\<close>], THEN spec[where x=\<open>Itself (v k)\<close>], THEN spec[where x=\<open>b * xc k\<close>],
           THEN mp, OF this]
     then show ?thesis
       apply clarsimp
@@ -182,12 +201,11 @@ lemma \<F>_pointwise_refinement:
           by (clarsimp simp add: sep_disj_fun_def prems2 prems(7)) (simp add: prems(7))
         have t3: \<open>1(k := b) * xc = u(k := v') * v\<close>
           by (clarsimp simp add: fun_eq_iff times_fun prems2,
-              metis (mono_tags, opaque_lifting) fun_upd_apply mult_1_class.mult_1_left prems(3) times_fun_def)
+              metis (mono_tags, opaque_lifting) fun_upd_apply mult_1_class.mult_1_left prems(5) times_fun)
         show ?thesis
           by (rule exI[where x=\<open>1(k := y)\<close>]; simp add: prems prems2; rule,
-              smt (verit, ccfv_threshold) fun_split_1 fun_upd_other fun_upd_same prems(5) prems(6) prems2(4) t3 t4 times_fun_def,
+              smt (verit, ccfv_SIG) fun_split_1 fun_upd_other fun_upd_same prems(3) prems(6) prems2(4) t3 t4 times_fun_def,
               metis fun_sep_disj_1_fupdt(2) fun_upd_triv prems2(1) prems2(2))
-              
       qed .
   qed .
 
@@ -258,7 +276,7 @@ lemma map_option_inj_at_1[simp]:
 
 lemma (in sep_orthogonal_monoid) \<F>_functional_projection:
   \<open> S \<le> D
-\<Longrightarrow> refinement_projection (\<F>_functional \<psi> D) (\<psi> `\<^sub>I S) \<le> S * top\<close>
+\<Longrightarrow> refinement_projection (\<F>_functional \<psi> D) (\<psi> ` S) \<le> S * top\<close>
   unfolding refinement_projection_def
   by (clarsimp simp add: subset_iff set_mult_expn eq_commute[where a=\<open>\<psi> _\<close>] sep_orthogonal; blast)
 
@@ -267,9 +285,9 @@ lemma \<F>_functional_pointwise:
   by (auto simp add: fun_eq_iff set_eq_iff; simp add: pointwise_set_def)
 
 lemma \<F>_functional_comp:
-  \<open> g ` Dg \<subseteq> Df
-\<Longrightarrow> \<F>_functional (f o g) Dg = \<F>_functional g Dg \<Zcomp>\<^sub>\<I> \<F>_functional f Df\<close>
-  by (auto simp add: fun_eq_iff set_eq_iff; blast)
+  \<open> g ` Dg \<le> Df
+\<Longrightarrow> \<F>_functional (f o g) Dg = (\<F>_functional g Dg \<Zcomp> \<F>_functional f Df)\<close>
+  by (auto simp add: fun_eq_iff BI_eq_iff)
   
 
 (* definition "\<F>_share s = (case s of Share w v \<Rightarrow> if w = 1 then {v} else {})"
@@ -302,15 +320,15 @@ lemma refinement_projection:
 subgoal for r R u v w *)
 
 definition \<F>_functional_condition
-  where \<open>\<F>_functional_condition D \<longleftrightarrow> (\<forall>r x y. x ## r \<and> y ## r \<and> r \<Turnstile> D \<and> x \<Turnstile> D \<and> x * r \<Turnstile> D \<and> y \<Turnstile> D \<longrightarrow> y * r \<Turnstile> D)\<close>
+  where \<open>\<F>_functional_condition D \<longleftrightarrow> (\<forall>r x y. x ## r \<and> y ## r \<and> r \<in> D \<and> x \<in> D \<and> x * r \<in> D \<and> y \<in> D \<longrightarrow> y * r \<in> D)\<close>
 
 lemma \<F>_functional_condition_UNIV[simp]:
   \<open>\<F>_functional_condition top\<close>
   unfolding \<F>_functional_condition_def by simp
 
-definition frame_preserving_relation \<comment> \<open>TODO: REALLY UGLY!\<close>
+definition frame_preserving_relation \<comment> \<open>TODO: UGLY?\<close>
   where \<open>frame_preserving_relation R
-    \<longleftrightarrow> (\<forall>a b c d r w. (a,b) \<Turnstile> R \<and> (c,d) \<Turnstile> R \<and> a * r = c * w \<and> a ## r \<and> b ## r \<and> c ## w
+    \<longleftrightarrow> (\<forall>a b c d r w. (a,b) \<in> R \<and> (c,d) \<in> R \<and> a * r = c * w \<and> a ## r \<and> b ## r \<and> c ## w
             \<longrightarrow> b * r = d * w \<and> d ## w)\<close>
 
 context cancl_sep_orthogonal_monoid begin
@@ -321,15 +339,15 @@ lemma \<F>_functional_refinement_complex:
 \<Longrightarrow> Sep_Closed D
 \<Longrightarrow> R * Id_on UNIV \<r>\<e>\<f>\<i>\<n>\<e>\<s> pairself \<psi> ` R \<w>.\<r>.\<t> \<F>_functional \<psi> D \<i>\<n> \<psi> ` (Domain R) \<close>
   unfolding Fictional_Forward_Simulation_def
-  apply (auto simp add: set_mult_expn Subjection_expn_set sep_orthogonal Sep_Closed_def image_iff Bex_def)
-  by (smt (z3) frame_preserving_relation_def homo_mult sep_disj_homo_semi sep_disj_multD1 sep_disj_multD2 sep_disj_multI1 sep_disj_multI2 sep_mult_assoc)
+  by (auto simp add: set_mult_expn sep_orthogonal Sep_Closed_def image_iff Bex_def,
+      smt (z3) frame_preserving_relation_def homo_mult sep_disj_homo_semi sep_disj_multD1 sep_disj_multD2 sep_disj_multI1 sep_disj_multI2 sep_mult_assoc)
 
 lemma \<F>_functional_refinement:
   \<open> a \<in> D \<and> b \<in> D
 \<Longrightarrow> \<F>_functional_condition D
 \<Longrightarrow> {(a, b)} * Id_on UNIV \<r>\<e>\<f>\<i>\<n>\<e>\<s> pairself \<psi> ` {(a,b)} \<w>.\<r>.\<t> \<F>_functional \<psi> D \<i>\<n> \<psi> ` {a} \<close>
   unfolding Fictional_Forward_Simulation_def \<F>_functional_condition_def
-  apply (auto simp add: set_mult_expn Subjection_expn_set sep_orthogonal)
+  apply (auto simp add: set_mult_expn sep_orthogonal)
   apply (metis (no_types, lifting) homo_mult sep_cancel sep_disj_multD1 sep_disj_multD2 sep_disj_multI1 sep_disj_multI2 sep_mult_assoc)
   by (metis sep_cancel sep_disj_homo_semi sep_disj_multD1 sep_disj_multD2 sep_disj_multI2 sep_mult_assoc)
 
