Phi_Semantics/PhiSem_Mem_C.thy
@@ -13,7 +13,7 @@ subsection \<open>Fiction\<close>
 type_synonym mem_fic = \<open>aggregate_path \<Rightarrow> VAL discrete share option\<close> \<comment> \<open>fiction of a single memory object\<close>
 
 fiction_space aggregate_mem =
-  aggregate_mem :: \<open>RES.aggregate_mem.basic_fiction \<Zcomp>\<^sub>\<I> \<F>_pointwise (\<lambda>blk. \<F>_functional ((\<circ>) to_share \<circ> Map_of_Val_ins) (Map_of_Val_ins_dom (memblk.layout blk)))\<close>
+  aggregate_mem :: \<open>RES.aggregate_mem.basic_fiction \<Zcomp> \<F>_pointwise (\<lambda>blk. \<F>_functional ((\<circ>) to_share \<circ> Map_of_Val_ins) (Map_of_Val_ins_dom (memblk.layout blk)))\<close>
      (perm_aggregate_mem_fiction RES.aggregate_mem memblk.layout Null)
   by (standard; simp)
 
